src/Init/Data/Nat/Basic.lean
@@ -620,6 +620,12 @@ theorem le_add_of_sub_le {a b c : Nat} (h : a - b ≤ c) : a ≤ c + b := by
     have hd := Nat.eq_add_of_sub_eq (Nat.le_trans hge (Nat.le_add_left ..)) hd
     rw [Nat.add_comm, hd]
 
+protected theorem sub_lt_sub_left : ∀ {k m n : Nat}, k < m → k < n → m - n < m - k
+  | 0, m+1, n+1, _, _ => by rw [Nat.add_sub_add_right]; exact lt_succ_of_le (Nat.sub_le _ _)
+  | k+1, m+1, n+1, h1, h2 => by
+    rw [Nat.add_sub_add_right, Nat.add_sub_add_right]
+    exact Nat.sub_lt_sub_left (Nat.lt_of_succ_lt_succ h1) (Nat.lt_of_succ_lt_succ h2)
+
 @[simp] protected theorem zero_sub (n : Nat) : 0 - n = 0 := by
   induction n with
   | zero => rfl
